src/CCL.v
@@ -1,3 +1,4 @@
 Require Export CCLProg CCLPrimitives CCLAutomation.
+Require Export Pred.
 Require Export CCLHashExec.
 Require Export CCLHoareTriples RetryLoop.
