src/OptimisticCache.v
@@ -1,6 +1,6 @@
 Require Import CCL.
 
-Require Import Mem Pred AsyncDisk.
+Require Import Mem AsyncDisk.
 Require Import MemCache.
 Require Import FunctionalExtensionality.
 Require Import UpdList.
